MathQL/MathQL/Expr.lean
@@ -1,0 +1,26 @@
+import MathQL.Name
+import MathQL.Operators
+import MathQL.Pattern
+
+namespace MathQL
+
+/-- Expressions -/
+inductive Expr where
+  | int : Int → Expr
+  | bool : Bool → Expr
+  | str : String → Expr
+  | enum : Ident → Expr
+  | var : Ident → Expr
+  | field : Expr → Label → Expr
+  | unop : UnaryOp → Expr → Expr
+  | binop : BinaryOp → Expr → Expr → Expr
+  | tuple : List Expr → Expr
+  | proj : Expr → Nat → Expr
+  | nil : Expr
+  | cons : Expr → Expr → Expr
+  | someE : Expr → Expr
+  | noneE : Expr
+  | ite : Expr → Expr → Expr → Expr
+  | bind : Pattern → Expr → Expr → Expr
+  | cases : Expr → List (Pattern × Expr) → Expr
+deriving Repr
