MathQL/MathQL/Name.lean
@@ -1,0 +1,9 @@
+namespace MathQL
+
+inductive Ident where
+  | ident : String → Ident
+deriving Repr, BEq, ReflBEq, LawfulBEq
+
+inductive Label where
+  | label : String → Label
+deriving Repr, BEq, ReflBEq, LawfulBEq
